loop_op correctness proved

nondeterministic_dataflow/Loop.thy
@@ -60,7 +60,9 @@ lemma loop_op_code[code]:
   subgoal for op' p' x
     by (subst loop_op.code) (auto 0 4 split: op.splits option.splits intro: loop_producing.intros)
   done
-simps_of_case loop_op_simps[simp]: loop_op_code
+simps_of_case loop_op_simps': loop_op_code
+simps_of_case loop_op_simps[simp]: loop_op.code[unfolded prod.case Let_def]
+
 
 section\<open>Correctness\<close>
 
@@ -86,21 +88,368 @@ lemma loop_producing_Some: "loop_producing wire buf op n \<Longrightarrow> wire 
       apply (auto simp: ran_def)
   done
 
-lemma loop_op_Some: "loop_op Some buf op = End"
+lemma not_loop_producing_eq_End: "\<forall>n. \<not> loop_producing wire buf op n \<Longrightarrow> loop_op wire buf op = End"
   apply (coinduction arbitrary: buf op)
   apply auto
   subgoal for buf op
     apply (subst (asm) loop_op.code)
-    apply (auto simp: ran_def dest: loop_producing_Some split: op.splits if_splits)
+    apply (auto split: op.splits if_splits option.splits simp: Let_def intro: loop_producing.intros)
     done
   subgoal for buf op
     apply (subst (asm) loop_op.code)
-    apply (auto simp: ran_def dest: loop_producing_Some split: op.splits if_splits)
+    apply (auto split: op.splits if_splits option.splits simp: Let_def intro: loop_producing.intros)
+    done
+  done
+
+lemma loop_op_Some: "loop_op Some buf op = End"
+  apply (coinduction arbitrary: buf op)
+  apply auto
+  subgoal for buf op
+    apply (cases op)
+      apply (simp_all add: ranI split: if_splits)
+    using loop_producing_Some not_loop_producing_eq_End apply blast+
+    done
+  subgoal for buf op
+    apply (cases op)
+      apply (simp_all add: ranI split: if_splits)
+    using loop_producing_Some not_loop_producing_eq_End apply blast+
+    done
+  done
+
+coinductive causal for wire where
+  "causal wire (BTL p buf) ios \<Longrightarrow> y = BHD p buf \<Longrightarrow> p \<in> ran wire \<Longrightarrow> causal wire buf (LCons (Inp p y) ios)"
+| "causal wire buf ios \<Longrightarrow> p \<notin> ran wire \<Longrightarrow> causal wire buf (LCons (Inp p y) ios)"
+| "causal wire (BENQ p' y buf) ios \<Longrightarrow> wire p = Some p' \<Longrightarrow> causal wire buf (LCons (Out p y) ios)"
+| "causal wire buf ios \<Longrightarrow> wire p = None \<Longrightarrow> causal wire buf (LCons (Out p y) ios)"
+| "causal wire buf LNil"
+
+inductive_cases causal_Inp[elim!]: "causal wire buf (LCons (Inp p y) ios)"
+inductive_cases causal_Out[elim!]: "causal wire buf (LCons (Out p y) ios)"
+inductive_cases causal_LNil[elim!]: "causal wire buf LNil"
+
+abbreviation visible_IO where "visible_IO wire io \<equiv> case_IO (\<lambda>p _. p \<notin> ran wire) (\<lambda> p _. p \<notin> dom wire) io" 
+
+lemma loop_producing_traced_causal_cong:
+  "loop_producing wire buf op n \<Longrightarrow>
+   traced op ios' \<Longrightarrow>
+   causal wire buf ios' \<Longrightarrow>
+   (\<exists>p f. loop_op wire buf op = Read p f \<and>
+          (\<exists>x lxs'.
+              lfilter (visible_IO wire) ios' = LCons (Inp p x) lxs' \<and>
+              traced_cong (\<lambda>opa lxs. \<exists>ios ios' op buf. opa = loop_op wire buf op \<and> lxs = ios \<and> traced op ios' \<and> ios = lfilter (visible_IO wire) ios' \<and> causal wire buf ios') (f x) lxs')) \<or>
+   (\<exists>op' q x.
+       loop_op wire buf op = Write op' q x \<and>
+       (\<exists>lxs'.
+           lfilter (visible_IO wire) ios' = LCons (Out q x) lxs' \<and>
+           traced_cong (\<lambda>opa lxs. \<exists>ios ios' op buf. opa = loop_op wire buf op \<and> lxs = ios \<and> traced op ios' \<and> ios = lfilter (visible_IO wire) ios' \<and> causal wire buf ios') op' lxs')) \<or>
+    loop_op wire buf op = End \<and> lfilter (visible_IO wire) ios' = LNil"
+  apply (induct  buf op n arbitrary: ios' rule: loop_producing.induct)
+  subgoal
+    by auto
+  subgoal
+    by (auto 10 10 intro: traced_cong.intros)
+  subgoal
+    apply (erule causal.cases)
+        apply (auto intro: traced_cong.intros)
+    done
+  subgoal
+    apply (erule causal.cases)
+        apply (auto intro: traced_cong.intros)
+    apply (meson loop_producing.intros(4))
+    done
+  subgoal
+    apply (erule causal.cases)
+        apply (auto intro: traced_cong.intros)
+      apply blast+
+    apply (meson loop_producing.intros(5))
+    done
+  done
+
+lemma in_traced_End_not_visible:
+  "x \<in> lset ios \<Longrightarrow> 
+   traced op ios \<Longrightarrow>
+   causal wire buf ios \<Longrightarrow>
+   loop_op wire buf op = End \<Longrightarrow>
+   \<not> visible_IO wire x"
+  apply (induct ios arbitrary: op buf rule: lset_induct)
+  subgoal for xs op buf
+    apply (cases op)
+      apply auto
+    done
+  subgoal for x' xs op buf
+    apply (cases op)
+      apply (auto split: if_splits)
+      apply (metis loop_op_simps'(1) loop_op_simps(1))
+     apply blast
+    apply (meson loop_producing.intros(5) not_loop_producing_eq_End)
+    done
+  done
+
+primcorec retrace_loop_op where
+  "retrace_loop_op wire buf op inps = (case op of
+     End \<Rightarrow> LNil
+   | Read p f \<Rightarrow> if p \<in> ran wire
+       then LCons (Inp p (BHD p buf)) (retrace_loop_op wire (BTL p buf) (f (BHD p buf)) inps)
+       else LCons (Inp p (lhd inps)) (retrace_loop_op wire buf (f (lhd inps)) (ltl inps))
+   | Write op' p' x \<Rightarrow> (case wire p' of
+         None \<Rightarrow> LCons (Out p' x) (retrace_loop_op wire buf op' inps)
+       | Some p \<Rightarrow> LCons (Out p' x) (retrace_loop_op wire (BENQ p x buf) op' inps)))"
+
+simps_of_case retrace_loop_op_simps[simp]: retrace_loop_op.code
+
+
+abbreviation "Inp_llist ios \<equiv> lmap (case_IO (\<lambda> p ob. ob) undefined) (lfilter (case_IO \<top> \<bottom>) ios)"
+
+lemma traced_retrace_loop_op:
+  "traced (loop_op wire buf op) ios \<Longrightarrow>
+   traced op (retrace_loop_op wire buf op (Inp_llist ios))"
+  apply (coinduction arbitrary: buf op ios)
+  subgoal for buf op ios
+    apply (cases op)
+    subgoal
+      apply (clarsimp simp add: lmap_eq_LNil split: if_splits; blast?)
+      apply (metis End lfilter_LNil lmap_eq_LNil loop_op_simps'(1) loop_op_simps(1))
+      done
+    subgoal
+      apply (clarsimp simp add: lmap_eq_LNil split: if_splits option.splits; blast?)
+      apply (metis (no_types, lifting) lfilter_LNil lmap_eq_LNil loop_op_simps'(2) not_loop_producing_eq_End option.simps(5) traced.simps)
+      done
+    subgoal
+      apply (clarsimp simp add: lmap_eq_LNil split: if_splits option.splits; blast?)
+      done
+    done
+  done
+
+
+lemma traced_retrace_loop_op_any[simp]:
+  "traced op (retrace_loop_op wire buf op inps)"
+  apply (coinduction arbitrary: op buf inps)
+  subgoal for op buf inps
+    apply (cases op)
+      apply (auto split: option.splits)
+    done
+  done
+
+lemma causal_retrace_loop_op[simp]:
+  "causal wire buf (retrace_loop_op wire buf op inps)"
+  apply (coinduction arbitrary: op buf inps)
+  subgoal for op buf inps
+   apply (cases op)
+      apply (auto split: option.splits)
+    done
+  done
+
+lemma retrace_loop_op_End_not_visible:
+  "x \<in> lset (retrace_loop_op wire buf op inps) \<Longrightarrow>
+   loop_op wire buf op = End \<Longrightarrow>
+   \<not> visible_IO wire x"
+  apply (induct "retrace_loop_op wire buf op inps" arbitrary: buf op inps rule: lset_induct)
+  subgoal for xs buf op inps
+    apply (cases op)
+      apply (auto split: if_splits option.splits)
+    done
+  subgoal for x' xs buf op inp
+    apply (cases op)
+      apply (simp_all split: if_splits option.splits)
+    subgoal
+      by (metis loop_op_simps'(1) loop_op_simps(1))
+    subgoal
+      by (metis loop_producing.intros(5) not_loop_producing_eq_End)
+    done
+  done
+
+lemma in_traced_loop_cases:
+  "loop_producing wire buf op n \<Longrightarrow>
+   traced (loop_op wire buf op) ios \<Longrightarrow>
+   loop_op wire buf op = End \<and> ios = LNil \<or>
+   (\<exists> op' x p buf'. loop_op wire buf op = Write (loop_op wire buf' op') p x \<and> lhd ios = Out p x \<and> wire p = None) \<or>
+   (\<exists> f x p buf'. loop_op wire buf op = Read p (\<lambda> x. loop_op wire buf' (f x)) \<and> lhd ios = Inp p x \<and> p \<notin> ran wire)"
+  apply (induct buf op n arbitrary: ios rule: loop_producing.induct)
+      apply (auto intro: End split: if_splits)
+  done
+
+lemma in_traced_loop_visible:
+  "x \<in> lset ios \<Longrightarrow>
+   traced (loop_op wire buf op) ios \<Longrightarrow>
+   visible_IO wire x"
+  apply (induct ios arbitrary: buf op rule: lset_induct)
+  subgoal for xs buf op
+    apply (cases "\<exists> n. loop_producing wire buf op n")
+    subgoal
+      apply (elim exE)
+      apply (frule in_traced_loop_cases)
+       apply auto
+      done
+    subgoal
+      by (metis llist.distinct(1) not_loop_producing_eq_End traced_EndE)
+    done
+  subgoal for x' xs buf op
+    apply (cases "\<exists> n. loop_producing wire buf op n")
+    subgoal
+      apply (elim exE)
+      apply (frule in_traced_loop_cases)
+       apply assumption
+      apply auto
+      done
+    subgoal
+      by (metis llist.distinct(1) not_loop_producing_eq_End traced_EndE)
+    done
+  done
+
+lemma loop_producing_traced_in_retrace_loop_op:
+  "loop_producing wire buf op n \<Longrightarrow>
+   x \<in> lset ios \<Longrightarrow>
+   traced (loop_op wire buf op) ios \<Longrightarrow>
+   \<exists> x. x \<in> lset (retrace_loop_op wire buf op (Inp_llist ios)) \<and> visible_IO wire x"
+  apply (induct buf op n arbitrary: ios rule: loop_producing.induct)
+      apply (fastforce split: if_splits option.splits)+
+  done 
+
+lemma traced_in_retrace_loop_op:
+  "x \<in> lset ios \<Longrightarrow>
+   traced (loop_op wire buf op) ios \<Longrightarrow>
+   \<exists> x. x \<in> lset (retrace_loop_op wire buf op (Inp_llist ios)) \<and> visible_IO wire x"
+  apply (cases "\<exists> n. loop_producing wire buf op n")
+  subgoal
+    by (auto dest: loop_producing_traced_in_retrace_loop_op)
+  subgoal
+    by (metis empty_iff lset_LNil not_loop_producing_eq_End traced_EndE)
+  done
+
+lemma loop_producing_traced_lhd_loop_producing:
+  "loop_producing wire buf op n \<Longrightarrow>
+   traced (loop_op wire buf op) (LCons io ios) \<Longrightarrow>
+   io = lhd (lfilter (visible_IO wire) (retrace_loop_op wire buf op (Inp_llist (LCons io ios))))"
+  apply (induct buf op n arbitrary: ios rule: loop_producing.induct)
+      apply (fastforce split: if_splits option.splits)+
+  done
+
+lemma traced_lhd_loop_producing:
+  "traced (loop_op wire buf op) (LCons io ios) \<Longrightarrow>
+   io = lhd (lfilter (visible_IO wire) (retrace_loop_op wire buf op (Inp_llist (LCons io ios))))"
+  apply (cases "\<exists> n. loop_producing wire buf op n")
+  subgoal
+    by (auto dest: loop_producing_traced_lhd_loop_producing)
+  subgoal
+    by (metis llist.simps(3) not_loop_producing_eq_End traced_EndE)
+  done
+
+lemma loop_producing_traced_cong:
+  "loop_producing wire buf op n \<Longrightarrow>
+   traced (loop_op wire buf op) ios \<Longrightarrow>
+   ios \<noteq> LNil \<Longrightarrow>
+   llist.v1.congclp
+    (\<lambda>llist llist'.
+        \<exists>buf op ios.
+           llist = ios \<and> llist' = lfilter (visible_IO wire) (retrace_loop_op wire buf op (Inp_llist ios)) \<and> traced (loop_op wire buf op) ios)
+    (ctl ios) (ctl (lfilter (visible_IO wire) (retrace_loop_op wire buf op (Inp_llist ios))))"
+  apply (induct buf op n arbitrary: ios rule: loop_producing.induct)
+      apply (force simp add:  observation.map_id split: if_splits option.splits intro!: llist.cong_LCons intro: llist.cong_base)+
+  done
+
+lemma traced_ios_lfilter_visible:
+  "traced (loop_op wire buf op) ios \<Longrightarrow>
+   ios = lfilter (visible_IO wire) (retrace_loop_op wire buf op (Inp_llist ios))"
+  apply (coinduction arbitrary: buf op ios rule: llist.coinduct_upto)
+  subgoal for buf op ios
+    apply (intro conjI impI iffI)
+    subgoal
+      by (auto simp add: lnull_def lmap_eq_LNil lfilter_eq_LNil dest: retrace_loop_op_End_not_visible)
+    subgoal
+      apply (simp add: lnull_def lmap_eq_LNil lfilter_eq_LNil)
+      apply (rule ccontr)
+      apply (clarsimp simp add: neq_LNil_conv)
+      apply (frule traced_in_retrace_loop_op[rotated 1]) 
+       apply auto
+      done
+    subgoal
+      unfolding lnull_def
+      apply (simp only: neq_LNil_conv)
+      apply (elim exE)
+      apply hypsubst_thin
+      apply (drule traced_lhd_loop_producing)
+      apply (metis lhd_LCons)
+      done
+    subgoal
+      apply (cases "\<exists> n. loop_producing wire buf op n")
+      subgoal
+        by (auto dest: loop_producing_traced_cong)
+      subgoal
+        by (metis lnull_def not_loop_producing_eq_End traced_EndE)
+      done
+    done
+  done
+
+lemma traced_loop_op:
+  "traced (loop_op wire buf op) ios =
+   (\<exists>ios'. traced op ios' \<and> ios = lfilter (visible_IO wire) ios' \<and> causal wire buf ios')"
+  apply (rule iffI)
+  subgoal 
+    apply (rule exI[of _ "retrace_loop_op wire buf op (Inp_llist ios)"])
+    apply (intro conjI)
+      apply (auto dest: traced_ios_lfilter_visible)
+    done
+  subgoal
+    apply (elim exE conjE)
+    subgoal for ios'
+      apply (coinduction arbitrary: ios ios' op buf rule: traced_coinduct_upto)
+      subgoal for ios ios' op buf
+        apply hypsubst_thin
+        apply (cases "\<exists> n. loop_producing wire buf op n")
+         apply (elim exE)
+        subgoal for n
+          apply (drule loop_producing_traced_causal_cong)
+            apply auto
+          done
+        subgoal
+          apply simp
+          apply (drule not_loop_producing_eq_End)
+          apply (auto simp add: lfilter_eq_LNil)
+          using in_traced_End_not_visible apply fast
+          done
+        done
+      done
     done
   done
 
 definition loop22_op :: "'d op22 \<Rightarrow> 'd op11" where
   "loop22_op op = map_op (\<lambda>_. 1) (\<lambda>_. 1) (loop_op
     (\<lambda>x. if x = 1 then Some 1 else None) (\<lambda>_. BEmpty) op)"
+
+corec Suc_op where
+  "Suc_op = Read (2::2) 
+            (case_observation 
+              (Write (Read 1 (case_observation (\<lambda> x. Write (Write Suc_op 1 (Suc x)) (2::2) (Suc x)) Suc_op Suc_op)) 1) Suc_op Suc_op)"
+
+abbreviation "loop_Suc_op buf \<equiv> loop_op
+    (\<lambda>x. if x = 1 then Some 1 else None) buf Suc_op"
+
+
+lemma
+  "history (loop_Suc_op (\<lambda> _. BCons 0 BEmpty)) (\<lambda> x. LNil) (\<lambda> x. if x = 2 then iterates Suc 0 else LNil)"
+  unfolding history_def
+  apply (simp add: traced_loop_op)
+  apply (rule exI[of _ "iterates (case_IO undefined (\<lambda> p n. Out p (Suc n))) (Out 2 0)"])
+  apply (intro conjI)
+  subgoal
+    apply (rule exI[of _ "retrace_loop_op (\<lambda>x. if x = 1 then Some 1 else None) (\<lambda>_. BCons 0 BEmpty) Suc_op LNil"])
+    apply (intro conjI)
+      apply (auto simp add: ran_def split: if_splits)
+    subgoal
+    apply (coinduction )
+    apply (intro conjI impI iffI)
+    subgoal
+      by auto
+    subgoal
+      apply (subst (asm) Suc_op.code)
+      apply (auto simp add: ran_def split: if_splits)
+      done
+    subgoal
+      unfolding lnull_def
+      apply (subst iterates.code)
+      apply simp
+      apply (subst Suc_op.code)
+      apply (simp add: ran_def)
+     oops
 
 end
